implement bir_valuesSyntax
rename BoolType -> BType_Bool which was forgotten previously

bir_valuesSyntax.sig
@@ -1,0 +1,121 @@
+signature bir_valuesSyntax =
+sig
+   include Abbrev
+
+   (*************)
+   (* bir_val_t *)
+   (*************)
+
+   (* The type itself *)
+   val bir_val_t_ty : hol_type
+
+   (* BVal_Unknown *)
+   val BVal_Unknown_tm : term
+   val is_BVal_Unknown : term -> bool
+
+   (* BVal_Imm *)
+   val BVal_Imm_tm   : term
+   val dest_BVal_Imm : term -> term
+   val is_BVal_Imm   : term -> bool
+   val mk_BVal_Imm   : term -> term
+
+   (* BVal_Mem *)
+   val BVal_Mem_tm   : term
+   val dest_BVal_Mem : term -> term * term * term
+   val is_BVal_Mem   : term -> bool
+   val mk_BVal_Mem   : term * term * term -> term
+
+   (* BVal_Imm for concrete sizes *)
+   val dest_BVal_Imm1    : term -> term
+   val dest_BVal_Imm8    : term -> term
+   val dest_BVal_Imm16   : term -> term
+   val dest_BVal_Imm32   : term -> term
+   val dest_BVal_Imm64   : term -> term
+   val gen_dest_BVal_Imm : term -> int * term
+
+   val is_BVal_Imm1    : term -> bool
+   val is_BVal_Imm8    : term -> bool
+   val is_BVal_Imm16   : term -> bool
+   val is_BVal_Imm32   : term -> bool
+   val is_BVal_Imm64   : term -> bool
+   val gen_is_BVal_Imm : int -> term -> bool
+
+
+   (* Memory that stores bytes is common, common
+      adderess sizes are 32 or 64 bit.
+      So let's provide special functions *)
+   val mk_BVal_MemByte   : term * term -> term
+   val dest_BVal_MemByte : term -> term * term
+   val is_BVal_MemByte   : term -> bool
+
+   val mk_BVal_MemByte_32   : term -> term
+   val dest_BVal_MemByte_32 : term -> term
+   val is_BVal_MemByte_32   : term -> bool
+
+   val mk_BVal_MemByte_64   : term -> term
+   val dest_BVal_MemByte_64 : term -> term
+   val is_BVal_MemByte_64   : term -> bool
+
+
+   (*****************)
+   (* bir_type_t    *)
+   (*****************)
+
+   (* The type itself *)
+   val bir_type_t_ty  : hol_type
+
+   (* BType_Imm *)
+   val BType_Imm_tm   : term
+   val dest_BType_Imm : term -> term
+   val is_BType_Imm   : term -> bool
+   val mk_BType_Imm   : term -> term
+
+   (* BType_Mem *)
+   val BType_Mem_tm   : term
+   val dest_BType_Mem : term -> term * term
+   val is_BType_Mem   : term -> bool
+   val mk_BType_Mem   : term * term -> term
+
+   (* BType_Imm special sizes *)
+   val gen_mk_BType_Imm   : int -> term
+   val gen_dest_BType_Imm : term -> int * term
+   val gen_is_BType_Imm   : int -> term -> bool
+
+   val BType_Imm1_tm  : term
+   val BType_Imm8_tm  : term
+   val BType_Imm16_tm : term
+   val BType_Imm32_tm : term
+   val BType_Imm64_tm : term
+
+   val is_BType_Imm1  : term -> bool
+   val is_BType_Imm8  : term -> bool
+   val is_BType_Imm16 : term -> bool
+   val is_BType_Imm32 : term -> bool
+   val is_BType_Imm64 : term -> bool
+
+   (* BType_Bool is defined as BType_Imm1, so let's have
+      a checker that recognizes both *)
+   val BType_Bool_tm  : term
+   val is_BType_Bool  : term -> bool
+   val is_BType_Bool_Imm1 : term -> bool
+
+
+   (* speical memory sizes *)
+   val mk_BType_MemByte    : term -> term
+   val dest_BType_MemByte  : term -> term
+   val is_BType_MemByte    : term -> bool
+
+   val BType_MemByte_32_tm : term
+   val BType_MemByte_64_tm : term
+
+
+   (***************************)
+   (* various functions       *)
+   (***************************)
+
+   val type_of_bir_val_tm   : term;
+   val mk_type_of_bir_val   : term -> term;
+   val dest_type_of_bir_val : term -> term;
+   val is_type_of_bir_val   : term -> bool;
+
+end
