selftest.sml
@@ -4,6 +4,6 @@ open HolBASimps birTheory;
 open bir_auxiliaryTheory bir_immTheory bir_valuesTheory;
 open bir_imm_expTheory bir_mem_expTheory bir_envTheory;
 open bir_expTheory bir_programTheory bir_typingTheory;
-open bir_immSyntax;
+open bir_immSyntax bir_valuesSyntax;
 
 val _ = Process.exit Process.success;
