birScript.sml
@@ -3,7 +3,7 @@ open wordsTheory bitstringTheory;
 open bir_auxiliaryTheory bir_immTheory bir_valuesTheory;
 open bir_imm_expTheory bir_mem_expTheory bir_envTheory;
 open bir_expTheory bir_programTheory bir_typingTheory;
-open bir_immSyntax;
+open bir_immSyntax bir_valuesSyntax;
 open wordsLib;
 
 val _ = new_theory "bir";
